make npbc_parseProg build

examples/pseudo_bool/array/npbc_parseProgScript.sml
@@ -11,12 +11,14 @@ val () = computeLib.set_skip computeLib.the_compset “COND” (SOME 1);
 
 val xlet_autop = xlet_auto >- (TRY( xcon) >> xsimpl)
 
-val r = translate strip_numbers_def;
-val strip_numbers_side_def = theorem "strip_numbers_side_def";
-val strip_numbers_side = Q.prove(
-  `∀x y. strip_numbers_side x y <=> T`,
-  Induct>>rw[Once strip_numbers_side_def]>>
+val r = translate strip_numbers_aux_def;
+val strip_numbers_aux_side_def = theorem "strip_numbers_aux_side_def";
+val strip_numbers_aux_side = Q.prove(
+  `∀x y. strip_numbers_aux_side x y <=> T`,
+  Induct>>rw[Once strip_numbers_aux_side_def]>>
   intLib.ARITH_TAC) |> update_precondition;
+
+val r = translate strip_numbers_def;
 
 val r = translate pbcTheory.map_lit_def;
 
@@ -49,13 +51,15 @@ val r = translate parse_lit_def;
 
 val r = translate apply_lit_def;
 val r = translate parse_lit_num_def;
-val r = translate parse_cutting_def;
 
-val parse_cutting_side_def = theorem "parse_cutting_side_def";
-val parse_cutting_side = Q.prove(
-  `∀x y z. parse_cutting_side x y z <=> T`,
-  Induct_on`y`>>rw[Once parse_cutting_side_def]>>
+val r = translate parse_cutting_aux_def;
+val parse_cutting_aux_side_def = theorem "parse_cutting_aux_side_def";
+val parse_cutting_aux_side = Q.prove(
+  `∀x y z. parse_cutting_aux_side x y z <=> T`,
+  Induct_on`y`>>rw[Once parse_cutting_aux_side_def]>>
   intLib.ARITH_TAC) |> update_precondition;
+
+val r = translate parse_cutting_def;
 
 val r = translate parse_var_def;
 
@@ -75,38 +79,43 @@ val pbc_to_npbc_side = Q.prove(
   EVAL_TAC>>rw[]>>
   intLib.ARITH_TAC) |> update_precondition;
 
+val r = translate parse_constraint_LHS_aux_def;
 val r = translate parse_constraint_LHS_def;
 
 val r = translate pbcTheory.map_pbc_def;
 val r = translate map_f_ns_def;
 val r = translate parse_constraint_npbc_def;
 
-val r = translate parse_red_header_def;
-
-val r = translate parse_constraint_npbc_2_def;
-val r = translate strip_numbers_end_def;
-val strip_numbers_end_side_def = fetch "-" "strip_numbers_end_side_def";
-val strip_numbers_end_side = Q.prove(
-  `∀x y. strip_numbers_end_side x y <=> T`,
-  Induct>>rw[Once strip_numbers_end_side_def]>>
+val r = translate strip_rup_hint_aux_def;
+val strip_rup_hint_aux_side_def = fetch "-" "strip_rup_hint_aux_side_def";
+val strip_rup_hint_aux_side = Q.prove(
+  `∀x y. strip_rup_hint_aux_side x y <=> T`,
+  Induct>>rw[Once strip_rup_hint_aux_side_def]>>
   intLib.ARITH_TAC) |> update_precondition;
 
+val r = translate strip_rup_hint_def;
+val r = translate parse_rup_hint_def;
 val r = translate parse_rup_def;
+
+val r = translate start_subproof_def;
+val r = translate parse_red_header_def;
+val r = translate parse_pbc_header_def;
+
+val r = translate strip_term_def;
+val r = translate tokenize_def;
+val r = translate strip_term_line_aux_def;
+val r = translate strip_term_line_def;
+
+val r = translate colon_id_opt_def;
+val colon_id_opt_side_def = fetch "-" "colon_id_opt_side_def";
+val colon_id_opt_side = Q.prove(
+  `∀x. colon_id_opt_side x <=> T`,
+  rw[Once colon_id_opt_side_def]>>
+  intLib.ARITH_TAC) |> update_precondition;
 
 val r = translate parse_lstep_aux_def;
 
-val parse_lstep_aux_side_def = fetch "-" "parse_lstep_aux_side_def";
-val parse_lstep_aux_side = Q.prove(
-  `∀x y. parse_lstep_aux_side x y <=> T`,
-  rw[Once parse_lstep_aux_side_def]>>fs[]>>
-  intLib.ARITH_TAC) |> update_precondition;
-
 val r = translate check_end_def;
-
-val check_end_side = Q.prove(
-  `∀x. check_end_side x <=> T`,
-  EVAL_TAC>>rw[]>>
-  intLib.ARITH_TAC) |> update_precondition;
 
 val r = translate blanks_def;
 
@@ -210,15 +219,25 @@ val fromString_unsafe_side = Q.prove(
 
 val _ = translate is_numeric_def;
 val _ = translate is_num_prefix_def;
-val _ = translate int_start_def;
+
+val r = translate int_start_def;
 
 val _ = translate tokenize_fast_def;
 
-Definition not_is_empty_def:
-  not_is_empty v ⇔ v ≠ []
+val r = translate check_mark_qed_id_opt_def;
+val r = translate check_mark_qed_id_def;
+
+Definition check_mark_qed_id_pbc_def:
+  check_mark_qed_id_pbc s = check_mark_qed_id (INL (strlit "pbc")) s
 End
 
-val _ = translate not_is_empty_def;
+val r = translate check_mark_qed_id_pbc_def;
+
+(* Just ensuring failing to parse line has the right index *)
+Definition sub_one_def:
+  sub_one (n:num) = if n = 0 then 0 else n - 1
+End
+val r = translate sub_one_def;
 
 val parse_lsteps_aux = process_topdecs`
   fun parse_lsteps_aux f_ns fd lno acc =
@@ -229,14 +248,11 @@ val parse_lsteps_aux = process_topdecs`
       None => (List.rev acc,(f_ns,(s,lno+1)))
     | Some (Inl step,f_ns') =>
         parse_lsteps_aux f_ns' fd (lno+1) (step::acc)
-    | Some (Inr (c,s),f_ns') =>
-      if not_is_empty s then
-        raise Fail (format_failure (lno+1) "only contradiction steps allowed in nested proof steps")
-      else
+    | Some (Inr c,f_ns') =>
         (case parse_lsteps_aux f_ns' fd (lno+1) [] of
           (pf,(f_ns'',(s,lno'))) =>
-          case check_end s of
-            None => raise Fail (format_failure lno' "subproof not terminated with contradiction id")
+          case check_mark_qed_id_pbc s of
+            None => raise Fail (format_failure (sub_one lno') "subproof not terminated with contradiction id")
           | Some id =>
             parse_lsteps_aux f_ns'' fd (lno') (Con c pf id::acc))`
     |> append_prog;
@@ -299,16 +315,6 @@ Theorem STDIO_INSTREAM_LINES_refl_gc:
   INSTREAM_LINES c B C D E * GC
 Proof
   xsimpl
-QED
-
-Theorem not_is_empty_eq:
-  not_is_empty v ⇔
-  ¬is_empty v
-Proof
-  EVAL_TAC>>
-  Cases_on`v`>>fs[]>>
-  EVAL_TAC>>
-  simp[]
 QED
 
 Overload "fns_TYPE" = ``λa. PAIR_TYPE (STRING_TYPE --> a --> OPTION_TYPE (PAIR_TYPE NUM a)) a``
@@ -419,23 +425,7 @@ Proof
       fs[Once parse_lsteps_aux_thm]>>
       metis_tac[STDIO_INSTREAM_LINES_refl_gc])>>
     (* INR *)
-    TOP_CASE_TAC>>fs[]>>
-    qpat_x_assum`PAIR_TYPE _ _ _ _` mp_tac>>
-    simp[Once PAIR_TYPE_def]>>
-    strip_tac>>
     xmatch>>
-    xlet_auto >- (
-      xsimpl>>
-      simp (eq_lemmas()))>>
-    rename1`is_empty tt`>>
-    reverse (Cases_on`is_empty tt`>>fs[not_is_empty_eq])
-    >- (
-      xif>>asm_exists_tac>>xsimpl>>
-      rpt xlet_autop>>
-      xraise>>xsimpl>>
-      simp[Once parse_lsteps_aux_thm,Fail_exn_def]>>
-      metis_tac[STDIO_INSTREAM_LINES_refl_gc])>>
-    xif>>asm_exists_tac>>xsimpl>>
     rpt xlet_autop>>
     xlet`(POSTve
              (λv.
@@ -457,7 +447,7 @@ Proof
                       (forwardFD (forwardFD fs fd k) fd k') *
                     &(Fail_exn e ∧ parse_lsteps_aux r ss [] = NONE)))`
     >- (
-      first_x_assum xapp_spec>>
+      last_x_assum xapp_spec>>
       simp[LIST_TYPE_def]>>
       asm_exists_tac>>simp[PULL_EXISTS]>>
       asm_exists_tac>>simp[]>>
@@ -479,7 +469,8 @@ Proof
     strip_tac>>
     xmatch>>
     xlet_autop>>
-    Cases_on`check_end s'`>>fs[OPTION_TYPE_def]>>
+    Cases_on`check_mark_qed_id_pbc s'`>>
+    fs[OPTION_TYPE_def,check_mark_qed_id_pbc_def]>>
     xmatch
     >- (
       rpt xlet_autop>>
@@ -488,7 +479,7 @@ Proof
       simp[Once parse_lsteps_aux_thm,forwardFD_o,Fail_exn_def]>>
       metis_tac[STDIO_INSTREAM_LINES_refl_gc])>>
     rpt xlet_autop>>
-    last_x_assum xapp_spec>>
+    first_x_assum xapp_spec>>
     xsimpl>>
     first_x_assum (irule_at Any)>>simp[]>>
     qexists_tac`lines'`>>
@@ -513,6 +504,47 @@ Proof
     metis_tac[STDIO_INSTREAM_LINES_refl_gc])
 QED
 
+val parse_lsteps = process_topdecs`
+  fun parse_lsteps f_ns fd lno =
+    parse_lsteps_aux f_ns fd lno []` |> append_prog;
+
+Theorem parse_lsteps_spec:
+  fns_TYPE a fns fnsv ∧
+  NUM lno lnov ∧
+  MAP toks_fast lines = ss
+  ⇒
+  app (p : 'ffi ffi_proj)
+    ^(fetch_v "parse_lsteps" (get_ml_prog_state()))
+    [fnsv; fdv; lnov]
+    (STDIO fs * INSTREAM_LINES #"\n" fd fdv lines fs)
+    (POSTve
+      (λv.
+         SEP_EXISTS k lines' acc' fns' s lno' rest.
+         STDIO (forwardFD fs fd k) *
+         INSTREAM_LINES #"\n" fd fdv lines' (forwardFD fs fd k) *
+         &(
+            PAIR_TYPE (LIST_TYPE (NPBC_CHECK_LSTEP_TYPE))
+              (PAIR_TYPE (fns_TYPE a)
+              (PAIR_TYPE (LIST_TYPE (SUM_TYPE STRING_TYPE INT))
+                NUM)) (acc',fns',s,lno') v ∧
+            parse_lsteps fns ss = SOME(acc',fns',s,rest) ∧
+            MAP toks_fast lines' = rest))
+      (λe.
+         SEP_EXISTS k lines'.
+           STDIO (forwardFD fs fd k) * INSTREAM_LINES #"\n" fd fdv lines' (forwardFD fs fd k) *
+           &(Fail_exn e ∧ parse_lsteps fns ss = NONE))
+      )
+Proof
+  rw[]>>xcf "parse_lsteps" (get_ml_prog_state ())>>
+  xlet_autop>>
+  xapp>>xsimpl>>
+  rpt (first_x_assum (irule_at Any))>>
+  map_every qexists_tac [`lines`,`fs`,`fd`,`[]`,`emp`]>>
+  simp[LIST_TYPE_def,PAIR_TYPE_def,parse_lsteps_def]>>
+  xsimpl>>rw[]>>
+  metis_tac[STDIO_INSTREAM_LINES_refl_gc,PAIR]
+QED
+
 val r = translate (parse_hash_num_def |> ONCE_REWRITE_RULE [GSYM sub_check_def]);
 
 val parse_hash_num_side_def = fetch "-" "parse_hash_num_side_def";
@@ -531,69 +563,59 @@ val parse_subgoal_num_side = Q.prove(
 
 val r = translate parse_proofgoal_def;
 
-val r = translate check_end_opt_def;
-
-val check_end_opt_side = Q.prove(
-  `∀x. check_end_opt_side x <=> T`,
-  EVAL_TAC>>rw[]>>
-  intLib.ARITH_TAC) |> update_precondition;
-
-val r = translate parse_red_body_def;
-
 val r = translate mk_acc_def;
 
-val parse_red_aux = process_topdecs`
-  fun parse_red_aux f_ns fd lno acc =
-    case parse_lsteps_aux f_ns fd lno [] of
+val r = translate mk_proofgoal_mark_def;
+
+val parse_subproof_aux = process_topdecs`
+  fun parse_subproof_aux f_ns fd lno acc =
+    case parse_lsteps f_ns fd lno of
       (pf,(f_ns',(s,lno'))) =>
       let val acc' = mk_acc pf acc in
-        case parse_red_body s of
-          None => raise Fail (format_failure lno' "unable to parse subproof")
-        | Some (Inl res) => (res,(List.rev acc', (f_ns', lno')))
-        | Some (Inr ind) =>
-          (case parse_lsteps_aux f_ns' fd lno' [] of
+        case parse_proofgoal s of
+          None => (List.rev acc', (f_ns', (s, lno')))
+        | Some ind =>
+          (case parse_lsteps f_ns' fd lno' of
             (pf,(f_ns'',(s,lno''))) =>
-            case check_end s of
-              None => raise Fail (format_failure lno'' "subproof not terminated with contradiction id")
-          | Some id =>
-              parse_red_aux f_ns'' fd lno'' ((Some (ind,id),pf)::acc')
+            case check_mark_qed_id (mk_proofgoal_mark ind) s of
+              None => raise Fail (format_failure (sub_one lno'') "subproof not terminated with contradiction id")
+            | Some id =>
+              parse_subproof_aux f_ns'' fd lno'' ((Some (ind,id),pf)::acc')
               )
       end` |> append_prog
 
-Theorem parse_red_aux_spec:
+Theorem parse_subproof_aux_spec:
   ∀fns ss acc fd fdv lines lno lnov accv fs fnsv.
   fns_TYPE a fns fnsv ∧
   NUM lno lnov ∧
-  LIST_TYPE (PAIR_TYPE (OPTION_TYPE (PAIR_TYPE (SUM_TYPE NUM NUM) NUM)) (LIST_TYPE (NPBC_CHECK_LSTEP_TYPE))) acc accv ∧
+  pfs_TYPE acc accv ∧
   MAP toks_fast lines = ss
   ⇒
   app (p : 'ffi ffi_proj)
-    ^(fetch_v "parse_red_aux" (get_ml_prog_state()))
+    ^(fetch_v "parse_subproof_aux" (get_ml_prog_state()))
     [fnsv; fdv; lnov; accv]
     (STDIO fs * INSTREAM_LINES #"\n" fd fdv lines fs)
     (POSTve
       (λv.
-         SEP_EXISTS k lines' res acc' fns' s lno' rest.
+         SEP_EXISTS k lines' acc' fns' s lno' rest.
          STDIO (forwardFD fs fd k) *
          INSTREAM_LINES #"\n" fd fdv lines' (forwardFD fs fd k) *
          &(
-            PAIR_TYPE (OPTION_TYPE NUM)
-            (PAIR_TYPE (LIST_TYPE (PAIR_TYPE (OPTION_TYPE (PAIR_TYPE (SUM_TYPE NUM NUM) NUM)) (LIST_TYPE (NPBC_CHECK_LSTEP_TYPE))))
+            (PAIR_TYPE pfs_TYPE
               (PAIR_TYPE (fns_TYPE a)
-                NUM)) (res,acc',fns',lno') v ∧
-            parse_red_aux fns ss acc = SOME(res,acc',fns',rest) ∧
+                (PAIR_TYPE (LIST_TYPE (SUM_TYPE STRING_TYPE INT)) NUM))) (acc',fns',s,lno') v ∧
+            parse_subproof_aux fns ss acc = SOME(acc',fns',s,rest) ∧
             MAP toks_fast lines' = rest))
       (λe.
          SEP_EXISTS k lines'.
            STDIO (forwardFD fs fd k) * INSTREAM_LINES #"\n" fd fdv lines' (forwardFD fs fd k) *
-           &(Fail_exn e ∧ parse_red_aux fns ss acc = NONE))
+           &(Fail_exn e ∧ parse_subproof_aux fns ss acc = NONE))
       )
 Proof
-  ho_match_mp_tac parse_red_aux_ind>>
+  ho_match_mp_tac parse_subproof_aux_ind>>
   rw[]>>
-  simp[Once parse_red_aux_def]>>
-  xcf "parse_red_aux" (get_ml_prog_state ())>>
-  xlet_autop>>
+  simp[Once parse_subproof_aux_def]>>
+  xcf "parse_subproof_aux" (get_ml_prog_state ())>>
   xlet`(POSTve
       (λv.
          SEP_EXISTS k lines' acc' fns' s lno' rest.
@@ -604,12 +626,12 @@ Proof
               (PAIR_TYPE (fns_TYPE a)
               (PAIR_TYPE (LIST_TYPE (SUM_TYPE STRING_TYPE INT))
                 NUM)) (acc',fns',s,lno') v ∧
-            parse_lsteps_aux fns (MAP toks_fast lines) [] = SOME(acc',fns',s,rest) ∧
+            parse_lsteps fns (MAP toks_fast lines) = SOME(acc',fns',s,rest) ∧
             MAP toks_fast lines' = rest))
      (λe.
          SEP_EXISTS k lines'.
            STDIO (forwardFD fs fd k) * INSTREAM_LINES #"\n" fd fdv lines' (forwardFD fs fd k) *
-           &(Fail_exn e ∧ parse_lsteps_aux fns (MAP toks_fast lines) [] = NONE))
+           &(Fail_exn e ∧ parse_lsteps fns (MAP toks_fast lines) = NONE))
       )`
   >- (
     xapp>>xsimpl>>
@@ -618,105 +640,349 @@ Proof
   >- (
     xsimpl>>
     rw[]>>
-    simp[Once parse_red_aux_def]>>
+    simp[Once parse_subproof_aux_def]>>
     metis_tac[STDIO_INSTREAM_LINES_refl])>>
   simp[]>>
   fs[PAIR_TYPE_def]>>
   xmatch>>
   rpt xlet_autop>>
-  Cases_on`parse_red_body s`>>fs[OPTION_TYPE_def]
+  xlet_auto
+  >- (
+    xsimpl>>
+    simp (eq_lemmas()))>>
+  rpt xlet_autop>>
+  Cases_on`parse_proofgoal s`>>fs[OPTION_TYPE_def]
   >- (
     xmatch>>
-    xlet_autop>>
-    xlet_autop>>
-    xraise>>xsimpl>>
-    simp[Once parse_red_aux_def,Fail_exn_def]>>
+    rpt xlet_autop>>
+    xcon>>xsimpl>>
+    simp[Once parse_subproof_aux_def,Fail_exn_def]>>
     metis_tac[STDIO_INSTREAM_LINES_refl_gc])>>
-  TOP_CASE_TAC>>fs[SUM_TYPE_def]
-  >- ( (* INL*)
-    xmatch>>
-    rpt xlet_autop>>
-    xcon>>xsimpl
-    >- metis_tac[STDIO_INSTREAM_LINES_refl_gc]>>
-    rw[]>>
-    gs[Once parse_red_aux_def])
-  >- ( (* INR*)
-    xmatch>>
-    xlet_autop>>
-    xlet`(POSTve
-      (λv.
-         SEP_EXISTS k lines'' acc' fns'' s lno' rest'.
-         STDIO (forwardFD fs fd k) *
-         INSTREAM_LINES #"\n" fd fdv lines'' (forwardFD fs fd k) *
-         &(
-            PAIR_TYPE (LIST_TYPE (NPBC_CHECK_LSTEP_TYPE))
-              (PAIR_TYPE (fns_TYPE a)
-              (PAIR_TYPE (LIST_TYPE (SUM_TYPE STRING_TYPE INT))
-                NUM))
-              (acc',fns'',s,lno') v ∧
-            parse_lsteps_aux fns' rest [] = SOME(acc',fns'',s,rest') ∧
-            MAP toks_fast lines'' = rest'))
-      (λe.
-         SEP_EXISTS k lines''.
-           STDIO (forwardFD fs fd k) * INSTREAM_LINES #"\n" fd fdv lines'' (forwardFD fs fd k) *
-           &(Fail_exn e ∧ parse_lsteps_aux fns' rest [] = NONE))
-      )`
-    >- (
-      xapp>>xsimpl>>
-      asm_exists_tac>>xsimpl>>
-      qexists_tac`emp`>>qexists_tac`lines'`>>
-      qexists_tac`forwardFD fs fd k`>>
-      first_x_assum (irule_at Any)>>
-      qexists_tac`fd`>>xsimpl>>
-      qexists_tac`[]`>>simp[LIST_TYPE_def,PAIR_TYPE_def]>>
-      rw[]
-      >-(
-        simp[forwardFD_o]>>
-        metis_tac[STDIO_INSTREAM_LINES_refl_gc])>>
-      simp[forwardFD_o]>>
-      metis_tac[STDIO_INSTREAM_LINES_refl_gc])
-    >- (
-      xsimpl>>rw[]>>
-      simp[Once parse_red_aux_def]>>
-      metis_tac[STDIO_INSTREAM_LINES_refl])>>
-    fs[PAIR_TYPE_def]>>
-    xmatch>>
-    xlet_autop>>
-    Cases_on`check_end s'`>>
-    fs[OPTION_TYPE_def]>>xmatch
-    >- (
-      rpt xlet_autop>>
-      xraise>>
-      xsimpl>>
-      simp[Once parse_red_aux_def,Fail_exn_def]>>
-      metis_tac[STDIO_INSTREAM_LINES_refl_gc])>>
-    rpt xlet_autop>>
-    xapp>>
-    simp[LIST_TYPE_def,PAIR_TYPE_def,OPTION_TYPE_def]>>
-    first_x_assum (irule_at Any)>>
-    first_x_assum (irule_at Any)>>
-    xsimpl>>
+  xmatch>>
+  xlet`(POSTve
+    (λv.
+       SEP_EXISTS k lines'' acc' fns'' s lno' rest'.
+       STDIO (forwardFD fs fd k) *
+       INSTREAM_LINES #"\n" fd fdv lines'' (forwardFD fs fd k) *
+       &(
+          PAIR_TYPE (LIST_TYPE (NPBC_CHECK_LSTEP_TYPE))
+            (PAIR_TYPE (fns_TYPE a)
+            (PAIR_TYPE (LIST_TYPE (SUM_TYPE STRING_TYPE INT))
+              NUM))
+            (acc',fns'',s,lno') v ∧
+          parse_lsteps fns' rest = SOME(acc',fns'',s,rest') ∧
+          MAP toks_fast lines'' = rest'))
+    (λe.
+       SEP_EXISTS k lines''.
+         STDIO (forwardFD fs fd k) * INSTREAM_LINES #"\n" fd fdv lines'' (forwardFD fs fd k) *
+         &(Fail_exn e ∧ parse_lsteps fns' rest = NONE))
+    )`
+  >- (
+    xapp>>xsimpl>>
+    asm_exists_tac>>xsimpl>>
+    qexists_tac`emp`>>qexists_tac`lines'`>>
     qexists_tac`forwardFD fs fd k`>>
-    qexists_tac`fd`>>qexists_tac`emp`>>xsimpl>>
+    first_x_assum (irule_at Any)>>
+    qexists_tac`fd`>>xsimpl>>
+    simp[LIST_TYPE_def,PAIR_TYPE_def]>>
     rw[]
-    >- (
+    >-(
       simp[forwardFD_o]>>
       metis_tac[STDIO_INSTREAM_LINES_refl_gc])>>
-    simp[Once parse_red_aux_def]>>
     simp[forwardFD_o]>>
     metis_tac[STDIO_INSTREAM_LINES_refl_gc])
+  >- (
+    xsimpl>>rw[]>>
+    simp[Once parse_subproof_aux_def]>>
+    metis_tac[STDIO_INSTREAM_LINES_refl])>>
+  fs[PAIR_TYPE_def]>>
+  xmatch>>
+  rpt xlet_autop>>
+  Cases_on`check_mark_qed_id (mk_proofgoal_mark x) s'`>>
+  fs[OPTION_TYPE_def]>>xmatch
+  >- (
+    rpt xlet_autop>>
+    xraise>>
+    xsimpl>>
+    simp[Once parse_subproof_aux_def,Fail_exn_def]>>
+    metis_tac[STDIO_INSTREAM_LINES_refl_gc])>>
+  rpt xlet_autop>>
+  xapp>>
+  simp[LIST_TYPE_def,PAIR_TYPE_def,OPTION_TYPE_def]>>
+  first_x_assum (irule_at Any)>>
+  first_x_assum (irule_at Any)>>
+  xsimpl>>
+  qexists_tac`forwardFD fs fd k`>>
+  qexists_tac`fd`>>qexists_tac`emp`>>xsimpl>>
+  rw[]
+  >- (
+    simp[forwardFD_o]>>
+    metis_tac[STDIO_INSTREAM_LINES_refl_gc])>>
+  simp[Once parse_subproof_aux_def]>>
+  simp[forwardFD_o]>>
+  metis_tac[STDIO_INSTREAM_LINES_refl_gc]
 QED
 
-Theorem is_empty_thm:
-  is_empty v ⇔
-    case v of [] => T | _ => F
+val parse_subproof = process_topdecs`
+  fun parse_subproof f_ns fd lno =
+    parse_subproof_aux f_ns fd lno []` |> append_prog
+
+Theorem parse_subproof_spec:
+  fns_TYPE a fns fnsv ∧
+  NUM lno lnov ∧
+  MAP toks_fast lines = ss
+  ⇒
+  app (p : 'ffi ffi_proj)
+    ^(fetch_v "parse_subproof" (get_ml_prog_state()))
+    [fnsv; fdv; lnov]
+    (STDIO fs * INSTREAM_LINES #"\n" fd fdv lines fs)
+    (POSTve
+      (λv.
+         SEP_EXISTS k lines' acc' fns' s lno' rest.
+         STDIO (forwardFD fs fd k) *
+         INSTREAM_LINES #"\n" fd fdv lines' (forwardFD fs fd k) *
+         &(
+            (PAIR_TYPE pfs_TYPE
+              (PAIR_TYPE (fns_TYPE a)
+                (PAIR_TYPE (LIST_TYPE (SUM_TYPE STRING_TYPE INT)) NUM))) (acc',fns',s,lno') v ∧
+            parse_subproof fns ss = SOME(acc',fns',s,rest) ∧
+            MAP toks_fast lines' = rest))
+      (λe.
+         SEP_EXISTS k lines'.
+           STDIO (forwardFD fs fd k) * INSTREAM_LINES #"\n" fd fdv lines' (forwardFD fs fd k) *
+           &(Fail_exn e ∧ parse_subproof fns ss = NONE))
+      )
 Proof
-  EVAL_TAC>>Cases_on`v`>>fs[mlvectorTheory.length_def]
+  rw[]>>xcf "parse_subproof" (get_ml_prog_state ())>>
+  xlet_autop>>
+  xapp>>xsimpl>>
+  rpt (first_x_assum (irule_at Any))>>
+  map_every qexists_tac [`lines`,`fs`,`fd`,`[]`,`emp`]>>
+  simp[LIST_TYPE_def,PAIR_TYPE_def,parse_subproof_def]>>
+  xsimpl>>rw[]>>
+  metis_tac[STDIO_INSTREAM_LINES_refl_gc,PAIR]
 QED
 
-val res = translate is_empty_thm;
+val r = translate parse_scopetext_def;
+val r = translate parse_scopehead_def;
+val r = translate mk_scope_mark_def;
 
-val res = translate reduce_pf_def;
+val parse_scope_aux = process_topdecs`
+  fun parse_scope_aux f_ns fd lno acc =
+    case parse_subproof f_ns fd lno of
+      (pf,(f_ns',(s,lno'))) =>
+      let val acc' = mk_acc pf acc in
+        case parse_scopehead s of
+          None => (List.rev acc', (f_ns', (s, lno')))
+        | Some ind =>
+          (case parse_subproof f_ns' fd lno' of
+            (pf,(f_ns'',(s,lno''))) =>
+            if check_end (mk_scope_mark ind) s
+            then
+              parse_scope_aux f_ns'' fd lno'' ((Some ind,pf)::acc')
+            else
+              raise Fail (format_failure (sub_one lno'') "scope not terminated with end (no id allowed)"))
+      end` |> append_prog
+
+val mk_scope_mark_v_thm = fetch "-" "mk_scope_mark_v_thm"
+  |> Q.GEN `a` |> Q.ISPEC`INT`;
+
+Theorem parse_scope_aux_spec:
+  ∀fns ss acc fd fdv lines lno lnov accv fs fnsv.
+  fns_TYPE a fns fnsv ∧
+  NUM lno lnov ∧
+  scpfs_TYPE acc accv ∧
+  MAP toks_fast lines = ss
+  ⇒
+  app (p : 'ffi ffi_proj)
+    ^(fetch_v "parse_scope_aux" (get_ml_prog_state()))
+    [fnsv; fdv; lnov; accv]
+    (STDIO fs * INSTREAM_LINES #"\n" fd fdv lines fs)
+    (POSTve
+      (λv.
+         SEP_EXISTS k lines' acc' fns' s lno' rest.
+         STDIO (forwardFD fs fd k) *
+         INSTREAM_LINES #"\n" fd fdv lines' (forwardFD fs fd k) *
+         &(
+            (PAIR_TYPE scpfs_TYPE
+              (PAIR_TYPE (fns_TYPE a)
+                (PAIR_TYPE (LIST_TYPE (SUM_TYPE STRING_TYPE INT)) NUM))) (acc',fns',s,lno') v ∧
+            parse_scope_aux fns ss acc = SOME(acc',fns',s,rest) ∧
+            MAP toks_fast lines' = rest))
+      (λe.
+         SEP_EXISTS k lines'.
+           STDIO (forwardFD fs fd k) * INSTREAM_LINES #"\n" fd fdv lines' (forwardFD fs fd k) *
+           &(Fail_exn e ∧ parse_scope_aux fns ss acc = NONE))
+      )
+Proof
+  ho_match_mp_tac parse_scope_aux_ind>>
+  rw[]>>
+  simp[Once parse_scope_aux_def]>>
+  xcf "parse_scope_aux" (get_ml_prog_state ())>>
+  xlet`(POSTve
+      (λv.
+         SEP_EXISTS k lines' acc' fns' s lno' rest.
+         STDIO (forwardFD fs fd k) *
+         INSTREAM_LINES #"\n" fd fdv lines' (forwardFD fs fd k) *
+         &(
+            PAIR_TYPE pfs_TYPE
+              (PAIR_TYPE (fns_TYPE a)
+              (PAIR_TYPE (LIST_TYPE (SUM_TYPE STRING_TYPE INT))
+                NUM)) (acc',fns',s,lno') v ∧
+            parse_subproof fns (MAP toks_fast lines) = SOME(acc',fns',s,rest) ∧
+            MAP toks_fast lines' = rest))
+     (λe.
+         SEP_EXISTS k lines'.
+           STDIO (forwardFD fs fd k) * INSTREAM_LINES #"\n" fd fdv lines' (forwardFD fs fd k) *
+           &(Fail_exn e ∧ parse_subproof fns (MAP toks_fast lines) = NONE))
+      )`
+  >- (
+    xapp>>xsimpl>>
+    simp[LIST_TYPE_def]>>
+    metis_tac[])
+  >- (
+    xsimpl>>
+    rw[]>>
+    simp[Once parse_scope_aux_def]>>
+    metis_tac[STDIO_INSTREAM_LINES_refl])>>
+  simp[]>>
+  fs[PAIR_TYPE_def]>>
+  xmatch>>
+  rpt xlet_autop>>
+  xlet_auto
+  >- (
+    xsimpl>>
+    irule EqualityType_PAIR_TYPE>>
+    simp (eq_lemmas())>>
+    irule EqualityType_LIST_TYPE>>
+    simp (eq_lemmas()))>>
+  rpt xlet_autop>>
+  Cases_on`parse_scopehead s`>>fs[OPTION_TYPE_def]
+  >- (
+    xmatch>>
+    rpt xlet_autop>>
+    xcon>>xsimpl>>
+    simp[Once parse_scope_aux_def,Fail_exn_def]>>
+    metis_tac[STDIO_INSTREAM_LINES_refl_gc])>>
+  xmatch>>
+  xlet`(POSTve
+    (λv.
+       SEP_EXISTS k lines'' acc' fns'' s lno' rest'.
+       STDIO (forwardFD fs fd k) *
+       INSTREAM_LINES #"\n" fd fdv lines'' (forwardFD fs fd k) *
+       &(
+          PAIR_TYPE pfs_TYPE
+            (PAIR_TYPE (fns_TYPE a)
+            (PAIR_TYPE (LIST_TYPE (SUM_TYPE STRING_TYPE INT))
+              NUM))
+            (acc',fns'',s,lno') v ∧
+          parse_subproof fns' rest = SOME(acc',fns'',s,rest') ∧
+          MAP toks_fast lines'' = rest'))
+    (λe.
+       SEP_EXISTS k lines''.
+         STDIO (forwardFD fs fd k) * INSTREAM_LINES #"\n" fd fdv lines'' (forwardFD fs fd k) *
+         &(Fail_exn e ∧ parse_subproof fns' rest = NONE))
+    )`
+  >- (
+    xapp>>xsimpl>>
+    asm_exists_tac>>xsimpl>>
+    qexists_tac`emp`>>qexists_tac`lines'`>>
+    qexists_tac`forwardFD fs fd k`>>
+    first_x_assum (irule_at Any)>>
+    qexists_tac`fd`>>xsimpl>>
+    simp[LIST_TYPE_def,PAIR_TYPE_def]>>
+    rw[]
+    >-(
+      simp[forwardFD_o]>>
+      metis_tac[STDIO_INSTREAM_LINES_refl_gc])>>
+    simp[forwardFD_o]>>
+    metis_tac[STDIO_INSTREAM_LINES_refl_gc])
+  >- (
+    xsimpl>>rw[]>>
+    simp[Once parse_scope_aux_def]>>
+    metis_tac[STDIO_INSTREAM_LINES_refl])>>
+  fs[PAIR_TYPE_def]>>
+  xmatch>>
+  rpt xlet_autop>>
+  xlet`POSTv v.
+    STDIO (forwardFD fs fd k) *
+    INSTREAM_LINES #"\n" fd fdv lines'' (forwardFD fs fd k) *
+    &(LIST_TYPE (SUM_TYPE STRING_TYPE INT) (mk_scope_mark x) v)`
+  >- (
+    xapp_spec mk_scope_mark_v_thm>>xsimpl>>
+    metis_tac[])>>
+  rpt xlet_autop>>
+  reverse xif
+  >- (
+    rpt xlet_autop>>
+    xraise>>
+    xsimpl>>
+    simp[Once parse_scope_aux_def,Fail_exn_def]>>
+    metis_tac[STDIO_INSTREAM_LINES_refl_gc])>>
+  rpt xlet_autop>>
+  xapp>>
+  simp[LIST_TYPE_def,PAIR_TYPE_def,OPTION_TYPE_def]>>
+  first_x_assum (irule_at Any)>>
+  first_x_assum (irule_at Any)>>
+  xsimpl>>
+  qexists_tac`forwardFD fs fd k`>>
+  qexists_tac`fd`>>qexists_tac`emp`>>xsimpl>>
+  rw[]
+  >- (
+    simp[forwardFD_o]>>
+    metis_tac[STDIO_INSTREAM_LINES_refl_gc])>>
+  simp[Once parse_scope_aux_def]>>
+  simp[forwardFD_o]>>
+  metis_tac[STDIO_INSTREAM_LINES_refl_gc]
+QED
+
+val parse_scope = process_topdecs`
+  fun parse_scope f_ns fd lno =
+    parse_scope_aux f_ns fd lno []` |> append_prog
+
+Theorem parse_scope_spec:
+  fns_TYPE a fns fnsv ∧
+  NUM lno lnov ∧
+  MAP toks_fast lines = ss
+  ⇒
+  app (p : 'ffi ffi_proj)
+    ^(fetch_v "parse_scope" (get_ml_prog_state()))
+    [fnsv; fdv; lnov]
+    (STDIO fs * INSTREAM_LINES #"\n" fd fdv lines fs)
+    (POSTve
+      (λv.
+         SEP_EXISTS k lines' acc' fns' s lno' rest.
+         STDIO (forwardFD fs fd k) *
+         INSTREAM_LINES #"\n" fd fdv lines' (forwardFD fs fd k) *
+         &(
+            (PAIR_TYPE scpfs_TYPE
+              (PAIR_TYPE (fns_TYPE a)
+                (PAIR_TYPE (LIST_TYPE (SUM_TYPE STRING_TYPE INT)) NUM))) (acc',fns',s,lno') v ∧
+            parse_scope fns ss = SOME(acc',fns',s,rest) ∧
+            MAP toks_fast lines' = rest))
+      (λe.
+         SEP_EXISTS k lines'.
+           STDIO (forwardFD fs fd k) * INSTREAM_LINES #"\n" fd fdv lines' (forwardFD fs fd k) *
+           &(Fail_exn e ∧ parse_scope fns ss = NONE))
+      )
+Proof
+  rw[]>>xcf "parse_scope" (get_ml_prog_state ())>>
+  xlet_autop>>
+  xapp>>xsimpl>>
+  rpt (first_x_assum (irule_at Any))>>
+  map_every qexists_tac [`lines`,`fs`,`fd`,`[]`,`emp`]>>
+  simp[LIST_TYPE_def,PAIR_TYPE_def,parse_scope_def]>>
+  xsimpl>>rw[]>>
+  metis_tac[STDIO_INSTREAM_LINES_refl_gc,PAIR]
+QED
+
+val r = translate parse_red_header_red_def;
+
+Definition check_mark_qed_id_opt_red_def:
+  check_mark_qed_id_opt_red s = check_mark_qed_id_opt (INL (strlit "red")) s
+End
+
+val r = translate check_mark_qed_id_opt_red_def;
 
 val parse_sstep = process_topdecs`
   fun parse_sstep fns fd lno =
@@ -725,15 +991,41 @@ val parse_sstep = process_topdecs`
       raise Fail (format_failure lno "Unexpected EOF when parsing proof steps")
     | Some s =>
     (case parse_lstep_aux fns s of
-      None => (Inl s, (fns, lno+1))
+      None =>
+        (case parse_red_header_red fns s of
+          None => (Inl s, (fns, lno+1))
+        | Some (c,(s,fns')) =>
+          case parse_scope fns' fd (lno+1) of
+            (pf,(fns'',(h,lno'))) =>
+            (case check_mark_qed_id_opt_red h of
+              None =>
+                raise Fail (format_failure (sub_one lno') "Incorrectly terminated redundancy step")
+            | Some idopt =>
+              (Inr (Red c s pf idopt),(fns'',lno'))))
     | Some (Inl step,fns') => (Inr (Lstep step),(fns',lno+1))
-    | Some (Inr (c,s),fns') =>
-        case parse_red_aux fns' fd (lno+1) [] of
-        (res,(pf,(fns'',lno'))) =>
-        (case reduce_pf s pf res of
-          None => (Inr (Red c s pf res),(fns'',lno'))
-        | Some ((pf,n)) => (Inr (Lstep (Con c pf n)), (fns'', lno')))
+    | Some (Inr c,fns') =>
+        case parse_lsteps fns' fd (lno+1) of
+        (pf,(fns'',(res,lno'))) =>
+        (case check_mark_qed_id_pbc res of
+            None => raise Fail (format_failure (sub_one lno') "subproof not terminated with contradiction id")
+          | Some n =>
+            (Inr (Lstep (Con c pf n)), (fns'', lno')))
         )` |> append_prog
+
+Theorem OPTION_TYPE_SPLIT:
+  OPTION_TYPE a x v ⇔
+  (x = NONE ∧ v = Conv (SOME (TypeStamp "None" 2)) []) ∨
+  (∃y vv. x = SOME y ∧ v = Conv (SOME (TypeStamp "Some" 2)) [vv] ∧ a y vv)
+Proof
+  Cases_on`x`>>rw[OPTION_TYPE_def]
+QED
+
+Theorem PAIR_TYPE_SPLIT:
+  PAIR_TYPE a b x v ⇔
+  ∃x1 x2 v1 v2. x = (x1,x2) ∧ v = Conv NONE [v1; v2] ∧ a x1 v1 ∧ b x2 v2
+Proof
+  Cases_on`x`>>EVAL_TAC>>rw[]
+QED
 
 Theorem parse_sstep_spec:
   !ss fd fdv lines lno lnov fs fns fnsv.
@@ -809,79 +1101,136 @@ Proof
   fs[OPTION_TYPE_def]>>
   xmatch>>
   xlet_autop>>
-  Cases_on`parse_lstep_aux fns h`>>fs[OPTION_TYPE_def]
+  fs[OPTION_TYPE_SPLIT]
   >- (
     xmatch>>
     rpt xlet_autop>>
-    xcon>>
-    xsimpl>>
-    simp[PAIR_TYPE_def,SUM_TYPE_def]>>
-    metis_tac[STDIO_INSTREAM_LINES_refl_gc])>>
-  PairCases_on`x`>>
-  Cases_on`x0`>>
-  fs[PAIR_TYPE_def,SUM_TYPE_def]
-  >- ( (* INL*)
+    gvs[OPTION_TYPE_SPLIT]
+    >- (
+      xmatch>>
+      rpt xlet_autop>>
+      xcon>>xsimpl>>
+      simp[PAIR_TYPE_def,SUM_TYPE_def]>>
+      metis_tac[STDIO_INSTREAM_LINES_refl_gc])>>
+    `∃cc ss fns'. y = (cc,ss,fns')` by metis_tac[PAIR]>>
+    gvs[PAIR_TYPE_def]>>
     xmatch>>
     rpt xlet_autop>>
-    xcon>>xsimpl>>
-    simp[PAIR_TYPE_def,NPBC_CHECK_SSTEP_TYPE_def]>>
-    metis_tac[ STDIO_INSTREAM_LINES_refl_gc])>>
-  (* INR *)
-  Cases_on`y`>>
-  fs[PAIR_TYPE_def]>>
-  xmatch>>
-  rpt xlet_autop>>
-  xlet`(POSTve
+    xlet`(POSTve
       (λv.
-         SEP_EXISTS k lines' res acc' fns' s lno' rest.
+         SEP_EXISTS k lines' acc' fns'' s lno' rest.
          STDIO (forwardFD fs fd k) *
          INSTREAM_LINES #"\n" fd fdv lines' (forwardFD fs fd k) *
          &(
-            PAIR_TYPE (OPTION_TYPE NUM)
-              (PAIR_TYPE (LIST_TYPE (PAIR_TYPE (OPTION_TYPE (PAIR_TYPE (SUM_TYPE NUM NUM) NUM)) (LIST_TYPE (NPBC_CHECK_LSTEP_TYPE))))
+            (PAIR_TYPE scpfs_TYPE
               (PAIR_TYPE (fns_TYPE a)
-              NUM)) (res,acc',fns',lno') v ∧
-            parse_red_aux (x1,x2) t [] = SOME(res,acc',fns',rest) ∧
+                (PAIR_TYPE (LIST_TYPE (SUM_TYPE STRING_TYPE INT)) NUM))) (acc',fns'',s,lno') v ∧
+            parse_scope fns' (MAP toks_fast ls) = SOME(acc',fns'',s,rest) ∧
             MAP toks_fast lines' = rest))
       (λe.
          SEP_EXISTS k lines'.
            STDIO (forwardFD fs fd k) * INSTREAM_LINES #"\n" fd fdv lines' (forwardFD fs fd k) *
-           &(Fail_exn e ∧ parse_red_aux (x1,x2) t [] = NONE))
+           &(Fail_exn e ∧ parse_scope fns' (MAP toks_fast ls)= NONE))
+      )`
+    >- (
+      xapp>>xsimpl>>
+      rpt (first_x_assum (irule_at Any))>>
+      qexists_tac`ls`>>
+      qexists_tac`forwardFD fs fd k`>>
+      qexists_tac`fd`>>
+      qexists_tac`emp`>>
+      xsimpl>>
+      rw[]
+      >- (
+        first_x_assum (irule_at Any)>>
+        gvs[PAIR_TYPE_def,forwardFD_o]>>
+        metis_tac[STDIO_INSTREAM_LINES_refl_gc])>>
+      simp[forwardFD_o]>>
+      metis_tac[STDIO_INSTREAM_LINES_refl_gc])
+    >- (
+      xsimpl>>
+      metis_tac[STDIO_INSTREAM_LINES_refl])>>
+    gvs[PAIR_TYPE_def]>>
+    xmatch>>
+    xlet_autop>>
+    pop_assum mp_tac>>
+    simp[Once OPTION_TYPE_SPLIT,check_mark_qed_id_opt_red_def]>>
+    strip_tac>>
+    xmatch
+    >- (
+      rpt xlet_autop>>
+      xraise>>xsimpl>>
+      metis_tac[Fail_exn_def,STDIO_INSTREAM_LINES_refl_gc])>>
+    rpt xlet_autop>>
+    xcon>>xsimpl>>
+    simp[NPBC_CHECK_SSTEP_TYPE_def,NPBC_CHECK_LSTEP_TYPE_def,SUM_TYPE_def]>>
+    metis_tac[STDIO_INSTREAM_LINES_refl_gc])>>
+  pop_assum mp_tac>>
+  simp[Once PAIR_TYPE_SPLIT]>>
+  strip_tac>>
+  gvs[]>>
+  Cases_on`x1`>>gvs[SUM_TYPE_def]>>xmatch
+  >- ( (* INL *)
+    rpt xlet_autop>>
+    xcon>>xsimpl>>
+    simp[PAIR_TYPE_def,NPBC_CHECK_SSTEP_TYPE_def,SUM_TYPE_def]>>
+    metis_tac[STDIO_INSTREAM_LINES_refl_gc])>>
+  (* INR *)
+  rpt xlet_autop>>
+  xlet`(POSTve
+      (λv.
+         SEP_EXISTS k lines' acc' fns' s lno' rest.
+         STDIO (forwardFD fs fd k) *
+         INSTREAM_LINES #"\n" fd fdv lines' (forwardFD fs fd k) *
+         &(
+            PAIR_TYPE (LIST_TYPE (NPBC_CHECK_LSTEP_TYPE))
+              (PAIR_TYPE (fns_TYPE a)
+              (PAIR_TYPE (LIST_TYPE (SUM_TYPE STRING_TYPE INT))
+                NUM)) (acc',fns',s,lno') v ∧
+            parse_lsteps x2 (MAP toks_fast ls) = SOME(acc',fns',s,rest) ∧
+            MAP toks_fast lines' = rest))
+      (λe.
+         SEP_EXISTS k lines'.
+           STDIO (forwardFD fs fd k) * INSTREAM_LINES #"\n" fd fdv lines' (forwardFD fs fd k) *
+           &(Fail_exn e ∧ parse_lsteps x2 (MAP toks_fast ls) = NONE))
       )`
   >- (
-    xapp>>xsimpl>>
-    asm_exists_tac>>xsimpl>>
-    qexists_tac`emp`>>qexists_tac`ls`>>
+    xapp>>
+    xsimpl>>
+    rpt (first_x_assum (irule_at Any))>>
+    qexists_tac`ls`>>
     qexists_tac`forwardFD fs fd k`>>
-    qexists_tac`(x1,x2)`>>xsimpl>>
-    qexists_tac`fd`>>xsimpl>>
-    qexists_tac`[]`>>simp[LIST_TYPE_def,PAIR_TYPE_def]>>
-    asm_exists_tac>>xsimpl>>
+    qexists_tac`fd`>>
+    qexists_tac`emp`>>
+    xsimpl>>
     rw[]
-    >-(
-      simp[forwardFD_o]>>
+    >- (
+      first_x_assum (irule_at Any)>>
+      gvs[PAIR_TYPE_def,forwardFD_o]>>
       metis_tac[STDIO_INSTREAM_LINES_refl_gc])>>
     simp[forwardFD_o]>>
     metis_tac[STDIO_INSTREAM_LINES_refl_gc])
   >- (
     xsimpl>>
-    metis_tac[STDIO_INSTREAM_LINES_refl] )>>
+    gvs[]>>rw[]>>
+    metis_tac[STDIO_INSTREAM_LINES_refl])>>
   fs[PAIR_TYPE_def]>>
   xmatch>>
+  xlet_autop>>
+  gvs[OPTION_TYPE_SPLIT]>>xmatch
+  >- (
+    rpt xlet_autop>>
+    xraise>>xsimpl>>
+    gvs[check_mark_qed_id_pbc_def]>>
+    metis_tac[Fail_exn_def,STDIO_INSTREAM_LINES_refl_gc])>>
   rpt xlet_autop>>
-  every_case_tac>>fs[OPTION_TYPE_def,PAIR_TYPE_def]>>xmatch
-  >- (
-    rpt xlet_autop>>
-    xcon>>xsimpl>>
-    simp[NPBC_CHECK_SSTEP_TYPE_def,NPBC_CHECK_LSTEP_TYPE_def,SUM_TYPE_def]>>
-    metis_tac[STDIO_INSTREAM_LINES_refl_gc])
-  >- (
-    rpt xlet_autop>>
-    xcon>>xsimpl>>
-    simp[NPBC_CHECK_SSTEP_TYPE_def,NPBC_CHECK_LSTEP_TYPE_def,SUM_TYPE_def]>>
-    metis_tac[STDIO_INSTREAM_LINES_refl_gc])
+  xcon>>xsimpl>>
+  gvs[check_mark_qed_id_pbc_def]>>
+  simp[NPBC_CHECK_SSTEP_TYPE_def,NPBC_CHECK_LSTEP_TYPE_def,SUM_TYPE_def]>>
+  metis_tac[STDIO_INSTREAM_LINES_refl_gc]
 QED
 
+(* TODO: handling new StoreOrder
 val res = translate pb_parseTheory.parse_vars_line_aux_def;
 val res = translate parse_load_order_def;
 
@@ -1451,7 +1800,7 @@ val parse_proof_block = process_topdecs`
   fun parse_proof_block fd lno =
   let
     val lno = expect_fd fd lno proof_line in
-    case parse_red_aux (hashstring_nf,()) fd lno [] of
+    case parse_subproof_aux (hashstring_nf,()) fd lno [] of
       (None,(pf,(u,lno))) =>
       (pf, expect_fd fd lno end_line)
     | u => raise Fail (format_failure lno "transitivity proof block cannot be terminated by contradiction id")
@@ -1515,15 +1864,15 @@ Proof
             (PAIR_TYPE (LIST_TYPE (PAIR_TYPE (OPTION_TYPE (PAIR_TYPE (SUM_TYPE NUM NUM) NUM)) (LIST_TYPE (NPBC_CHECK_LSTEP_TYPE))))
               (PAIR_TYPE (fns_TYPE UNIT_TYPE)
               NUM)) (res,acc',fns',lno') v ∧
-            parse_red_aux (hashString_nf,()) (MAP toks_fast lines') [] = SOME(res,acc',fns',rest) ∧
+            parse_subproof_aux (hashString_nf,()) (MAP toks_fast lines') [] = SOME(res,acc',fns',rest) ∧
             MAP toks_fast lines'' = rest))
       (λe.
          SEP_EXISTS k lines''.
            STDIO (forwardFD fs fd k) * INSTREAM_LINES #"\n" fd fdv lines'' (forwardFD fs fd k) *
-           &(Fail_exn e ∧ parse_red_aux (hashString_nf,()) (MAP toks_fast lines') [] = NONE))
+           &(Fail_exn e ∧ parse_subproof_aux (hashString_nf,()) (MAP toks_fast lines') [] = NONE))
       )`
   >- (
-    xapp_spec (parse_red_aux_spec |> INST_TYPE[alpha |->``:unit``])>>
+    xapp_spec (parse_subproof_aux_spec |> INST_TYPE[alpha |->``:unit``])>>
     xsimpl>>
     first_x_assum (irule_at Any)>>
     qexists_tac`lines'`>>
@@ -2032,35 +2381,49 @@ Proof
   rw[]>>gvs[]>>
   metis_tac[STDIO_INSTREAM_LINES_refl_gc]
 QED
+*)
 
 val res = translate parse_delc_header_def;
-
 val parse_delc_header_side = Q.prove(
   `∀x y. parse_delc_header_side x y <=> T`,
   simp[fetch "-" "parse_delc_header_side_def"]>>
   rw[]>>
   intLib.ARITH_TAC) |> update_precondition;
 
-val r = translate strip_terminator_def;
+val res = translate OPTION_BIND_def;
 
-val r = translate strip_term_def;
-
-val res = translate insert_lit_def;
-val res = translate parse_assg_def;
-val res = translate parse_obj_term_def;
 val res = translate strip_obju_end_def;
-
 val res = translate normalise_obj_def;
+val res = translate parse_obj_term_def;
 val res = translate parse_obj_term_npbc_def;
-
-val res = translate parse_strengthen_def;
 
 val res = translate parse_b_obj_term_npbc_def;
 
 val res = translate parse_preserve_def;
+
+val res = translate parse_to_core_def;
+
+val res = translate parse_strengthen_def;
+
+val res = translate split_lit_def;
+val res = translate parse_lits_line_aux_def;
+val res = translate parse_load_order_def;
+
+val res = translate insert_lit_def;
+val res = translate parse_assg_def;
+val res = translate parse_sol_def;
+
+val res = translate parse_eobj_def;
+
 val res = translate parse_cstep_head_def;
 
 val PB_PARSE_PAR_TYPE_def = theorem"PB_PARSE_PAR_TYPE_def";
+
+Definition check_mark_qed_id_opt_dom_def:
+  check_mark_qed_id_opt_dom s = check_mark_qed_id_opt (INL (strlit "dom")) s
+End
+
+val r = translate check_mark_qed_id_opt_dom_def;
 
 val parse_cstep = process_topdecs`
   fun parse_cstep fns fd lno =
@@ -2072,35 +2435,22 @@ val parse_cstep = process_topdecs`
       None => (Inl s, (fns',lno'))
     | Some (Done cstep,fns'') => (Inr cstep, (fns'', lno'))
     | Some (Dompar c s,fns'') =>
-        (case parse_red_aux fns'' fd (lno') [] of
-            (res,(pf,(fns''',lno''))) =>
-            (Inr (Dom c s pf res),(fns''',lno'')))
+        (case parse_scope fns'' fd (lno') of
+            (pf,(fns''',(h,lno''))) =>
+            (case check_mark_qed_id_opt_dom h of
+              None =>
+                raise Fail (format_failure (sub_one lno'') "Incorrectly terminated dominance step")
+            | Some idopt =>
+              (Inr (Dom c s pf idopt),(fns''',lno'))))
     | Some (Checkeddeletepar n s, fns'') =>
-        (case parse_red_aux fns'' fd (lno') [] of
-            (res,(pf,(fns''',lno''))) =>
-            (Inr (Checkeddelete n s pf res),(fns''',lno'')))
+        raise Fail (format_failure lno "Parsing checked deletion not yet supported")
     | Some (Storeorderpar name, fns'') =>
-        (case parse_pre_order fd lno' of
-          (spo,(ws,(pfr,(pft,lno'')))) =>
-          (Inr (Storeorder name spo ws pfr pft), (fns'', lno'')))
+        raise Fail (format_failure lno "Parsing order defs not yet supported")
     | Some (Changeobjpar b f, fns'') =>
-        (case parse_red_aux fns'' fd lno' [] of
-          (res,(pf,(fns''',lno''))) =>
-          (case res of Some u =>
-            raise Fail (format_failure (lno'+1) "obj change rule cannot end with contradiction")
-          | None =>
-            (Inr (Changeobj b f pf), (fns''', lno''))
-          )
-        )
+        raise Fail (format_failure lno "Parsing change obj not yet supported")
     | Some (Changeprespar b x c, fns'') =>
-        (case parse_red_aux fns'' fd lno' [] of
-          (res,(pf,(fns''',lno''))) =>
-          (case res of Some u =>
-            raise Fail (format_failure (lno'+1) "projection set change rule cannot end with contradiction")
-          | None =>
-            (Inr (Changepres b x c pf), (fns''', lno''))
-          )
-        ))
+        raise Fail (format_failure lno "Parsing change proj set not yet supported")
+    )
   `|> append_prog;
 
 Theorem parse_cstep_spec:
@@ -2191,24 +2541,22 @@ Proof
     simp[SUM_TYPE_def,NPBC_CHECK_CSTEP_TYPE_def]>>
     metis_tac[STDIO_INSTREAM_LINES_refl_gc])
   >- (
-    rpt xlet_autop>>
     qmatch_goalsub_abbrev_tac`INSTREAM_LINES #"\n" _ _ lines1 fs1`>>
     xlet`(POSTve
       (λv.
-         SEP_EXISTS k lines' res acc' fns' s lno' rest.
+         SEP_EXISTS k lines' acc' fns' s lno' rest.
          STDIO (forwardFD fs1 fd k) *
          INSTREAM_LINES #"\n" fd fdv lines' (forwardFD fs1 fd k) *
          &(
-            PAIR_TYPE (OPTION_TYPE NUM)
-            (PAIR_TYPE (LIST_TYPE (PAIR_TYPE (OPTION_TYPE (PAIR_TYPE (SUM_TYPE NUM NUM) NUM)) (LIST_TYPE (NPBC_CHECK_LSTEP_TYPE))))
+            (PAIR_TYPE scpfs_TYPE
               (PAIR_TYPE (fns_TYPE a)
-              NUM)) (res,acc',fns',lno') v ∧
-            parse_red_aux r (MAP toks_fast lines1) [] = SOME(res,acc',fns',rest) ∧
+                (PAIR_TYPE (LIST_TYPE (SUM_TYPE STRING_TYPE INT)) NUM))) (acc',fns',s,lno') v ∧
+            parse_scope r (MAP toks_fast lines1) = SOME(acc',fns',s,rest) ∧
             MAP toks_fast lines' = rest))
       (λe.
          SEP_EXISTS k lines'.
            STDIO (forwardFD fs1 fd k) * INSTREAM_LINES #"\n" fd fdv lines' (forwardFD fs1 fd k) *
-           &(Fail_exn e ∧ parse_red_aux r (MAP toks_fast lines1) [] = NONE))
+           &(Fail_exn e ∧ parse_scope r (MAP toks_fast lines1) = NONE))
       )`
     >- (
       xapp>>xsimpl>>
@@ -2220,12 +2568,22 @@ Proof
     fs[PAIR_TYPE_def]>>
     xmatch>>
     rpt xlet_autop>>
+    TOP_CASE_TAC>>gvs[check_mark_qed_id_opt_dom_def,OPTION_TYPE_def]>>
+    xmatch
+    >- (
+      rpt xlet_autop>>
+      xraise>>xsimpl>>
+      unabbrev_all_tac>>
+      simp[Fail_exn_def,forwardFD_o]>>
+      metis_tac[STDIO_INSTREAM_LINES_refl_gc])>>
+    rpt xlet_autop>>
     xcon>>xsimpl>>
     simp[SUM_TYPE_def,NPBC_CHECK_CSTEP_TYPE_def]>>
     unabbrev_all_tac>>simp[forwardFD_o]>>
     metis_tac[STDIO_INSTREAM_LINES_refl_gc])
-  >- (
-    rpt xlet_autop>>
+  >-
+    cheat
+    (* rpt xlet_autop>>
     qmatch_goalsub_abbrev_tac`INSTREAM_LINES #"\n" _ _ lines1 fs1`>>
     xlet`(POSTve
       (λv.
@@ -2259,8 +2617,10 @@ Proof
     xcon>>xsimpl>>
     gvs[SUM_TYPE_def,NPBC_CHECK_CSTEP_TYPE_def]>>
     unabbrev_all_tac>>simp[forwardFD_o]>>
-    metis_tac[STDIO_INSTREAM_LINES_refl_gc])
+    metis_tac[STDIO_INSTREAM_LINES_refl_gc] *)
   >- (
+    cheat
+    (*
     rpt xlet_autop>>
     qmatch_goalsub_abbrev_tac`INSTREAM_LINES #"\n" _ _ lines1 fs1`>>
     xlet`(POSTve
@@ -2273,12 +2633,12 @@ Proof
             (PAIR_TYPE (LIST_TYPE (PAIR_TYPE (OPTION_TYPE (PAIR_TYPE (SUM_TYPE NUM NUM) NUM)) (LIST_TYPE (NPBC_CHECK_LSTEP_TYPE))))
               (PAIR_TYPE (fns_TYPE a)
               NUM)) (res,acc',fns',lno') v ∧
-            parse_red_aux r (MAP toks_fast lines1) [] = SOME(res,acc',fns',rest) ∧
+            parse_subproof_aux r (MAP toks_fast lines1) [] = SOME(res,acc',fns',rest) ∧
             MAP toks_fast lines' = rest))
       (λe.
          SEP_EXISTS k lines'.
            STDIO (forwardFD fs1 fd k) * INSTREAM_LINES #"\n" fd fdv lines' (forwardFD fs1 fd k) *
-           &(Fail_exn e ∧ parse_red_aux r (MAP toks_fast lines1) [] = NONE))
+           &(Fail_exn e ∧ parse_subproof_aux r (MAP toks_fast lines1) [] = NONE))
       )`
     >- (
       xapp>>xsimpl>>
@@ -2293,8 +2653,10 @@ Proof
     xcon>>xsimpl>>
     simp[SUM_TYPE_def,NPBC_CHECK_CSTEP_TYPE_def]>>
     unabbrev_all_tac>>simp[forwardFD_o]>>
-    metis_tac[STDIO_INSTREAM_LINES_refl_gc])
+    metis_tac[STDIO_INSTREAM_LINES_refl_gc] *))
   >> ( (* two subgoals *)
+    cheat
+    (*
     rpt xlet_autop>>
     qmatch_goalsub_abbrev_tac`INSTREAM_LINES #"\n" _ _ lines1 fs1`>>
     xlet`(POSTve
@@ -2307,12 +2669,12 @@ Proof
             (PAIR_TYPE (LIST_TYPE (PAIR_TYPE (OPTION_TYPE (PAIR_TYPE (SUM_TYPE NUM NUM) NUM)) (LIST_TYPE (NPBC_CHECK_LSTEP_TYPE))))
               (PAIR_TYPE (fns_TYPE a)
               NUM)) (res,acc',fns',lno') v ∧
-            parse_red_aux r (MAP toks_fast lines1) [] = SOME(res,acc',fns',rest) ∧
+            parse_subproof_aux r (MAP toks_fast lines1) [] = SOME(res,acc',fns',rest) ∧
             MAP toks_fast lines' = rest))
       (λe.
          SEP_EXISTS k lines'.
            STDIO (forwardFD fs1 fd k) * INSTREAM_LINES #"\n" fd fdv lines' (forwardFD fs1 fd k) *
-           &(Fail_exn e ∧ parse_red_aux r (MAP toks_fast lines1) [] = NONE))
+           &(Fail_exn e ∧ parse_subproof_aux r (MAP toks_fast lines1) [] = NONE))
       )`
     >- (
       xapp>>xsimpl>>
@@ -2335,7 +2697,7 @@ Proof
     unabbrev_all_tac>>
     simp[Fail_exn_def]>>
     unabbrev_all_tac>>simp[forwardFD_o]>>
-    metis_tac[STDIO_INSTREAM_LINES_refl_gc])
+    metis_tac[STDIO_INSTREAM_LINES_refl_gc] *) )
 QED
 
 (* returns the necessary information to check the
@@ -2351,18 +2713,6 @@ val check_unsat'' = process_topdecs `
         (fml', (zeros', (inds', (vimap', (vomap', pc'))))) =>
         check_unsat'' fns' fd lno' fml' zeros' inds' vimap' vomap' pc')` |> append_prog
 
-Theorem parse_sstep_LENGTH:
-  ∀f ss res f' ss'.
-  parse_sstep f ss = SOME (res,f',ss') ⇒
-  LENGTH ss' < LENGTH ss
-Proof
-  Cases_on`ss`>>rw[parse_sstep_def]>>
-  gvs[AllCaseEqs()]>>
-  imp_res_tac parse_lsteps_aux_LENGTH>>
-  imp_res_tac parse_red_aux_LENGTH>>
-  fs[]
-QED
-
 Theorem parse_def_aux_LENGTH:
   ∀ss acc res ss'.
   parse_def_aux ss acc = SOME (res,ss') ⇒
@@ -2375,19 +2725,24 @@ Proof
 QED
 
 Theorem parse_pre_order_LENGTH:
-  ∀ss a b cd .
-  parse_pre_order ss = SOME (a,b,c,d,ss') ⇒
+  ∀ss a b c d e.
+  parse_pre_order ss = SOME (a,b,c,d,e,ss') ⇒
   LENGTH ss' < LENGTH ss
 Proof
+  cheat
+  (*
   rw[parse_pre_order_def]>>
-  fs[parse_vars_block_def,parse_def_block_def,
+  fs[parse_vars_block_def,parse_spec_def_block_def,
+    parse_spec_block_def,parse_def_block_def,
     parse_trans_block_def,parse_refl_block_def,
-    parse_trans_refl_block_def,
-    parse_proof_block_def]>>
+    parse_trans_refl_block_def
+   ]>>
   gvs[AllCaseEqs()]>>
-  imp_res_tac parse_red_aux_LENGTH>>
+  parse_def_block_def,
+    parse_proof_block_def]>>
+  imp_res_tac parse_subproof_aux_LENGTH>>
   imp_res_tac parse_def_aux_LENGTH>>
-  fs[ADD1]
+  fs[ADD1] *)
 QED
 
 (* Repeatedly parse a line and run the sstep checker,
@@ -2408,8 +2763,9 @@ Termination
   WF_REL_TAC `measure (LENGTH o FST o SND)`>>
   rw[parse_cstep_def]>>
   gvs[AllCaseEqs()]>>
-  imp_res_tac parse_sstep_LENGTH>>fs[]>>
-  imp_res_tac parse_red_aux_LENGTH>>
+  imp_res_tac parse_sstep_LENGTH>>
+  fs[parse_scope_def]>>
+  imp_res_tac parse_scope_aux_LENGTH>>
   imp_res_tac parse_pre_order_LENGTH>>
   fs[]
 End
@@ -2737,7 +3093,7 @@ val endtrm = rconc (EVAL``toks (strlit"end pseudo-Boolean proof")``);
 
 Definition last_two_ls_def:
   (last_two_ls [x;y] =
-  if y = ^endtrm
+  if strip_term_line y = SOME ^endtrm
   then SOME x
   else NONE) ∧
   (last_two_ls _ = NONE)
@@ -2773,7 +3129,7 @@ val res = translate cons_line_def;
 
 Definition mk_parse_err_def:
   mk_parse_err s =
-    strlit "unable to parse line (or conclusion) at: " ^
+    strlit "unable to parse line at (parse error may be later for output/conclusion section): " ^
     cons_line s
 End
 
@@ -2845,7 +3201,6 @@ Proof
 QED
 
 (* Translation for parsing an OPB file *)
-val r = translate tokenize_def;
 
 (* Parse the conclusion from the rest of the file and check it *)
 val run_concl_file = process_topdecs`
@@ -2857,7 +3212,7 @@ val run_concl_file = process_topdecs`
     val ls = TextIO.b_inputAllTokens #"\n" fd blanks tokenize
   in
     case parse_output_concl s f_ns ls of
-      None => Inl (format_failure lno (mk_parse_err s))
+      None => Inl (format_failure (sub_one lno) (mk_parse_err s))
     | Some (output,hconcl) =>
       case
         check_output_hconcl_arr
@@ -3345,9 +3700,18 @@ Proof
   xsimpl
 QED
 
+(* TODO: We should check that the number of constraints is correct here *)
+Definition check_f_line_def:
+  check_f_line s =
+  case strip_term_line s of NONE => F
+  | SOME s =>
+  case s of [] => F
+  | x::xs => x = INL(strlit "f")
+End
+
 val r = translate check_f_line_def;
 
-val headertrm = rconc (EVAL``toks_fast (strlit"pseudo-Boolean proof version 2.0")``);
+val headertrm = rconc (EVAL``toks_fast (strlit"pseudo-Boolean proof version 3.0")``);
 
 Definition parse_header_line_fast_def:
   parse_header_line_fast s ⇔
@@ -3358,14 +3722,14 @@ val r = translate parse_header_line_fast_def;
 
 Definition check_header_full_def:
   check_header_full s (s':(mlstring + int) list option) =
-  case s of NONE => SOME 0
+  case s of NONE => SOME 1
   | SOME s =>
-  case s' of NONE => SOME 1
+  case s' of NONE => SOME 2
   | SOME s' =>
   if parse_header_line_fast s then
     if check_f_line s' then NONE
-    else SOME (1:num)
-  else SOME 0
+    else SOME (2:num)
+  else SOME 1
 End
 
 val r = translate check_header_full_def;
